added spinlock well-sync and spinlock clean definitions

concurrency/x86_safe.v
@@ -46,7 +46,35 @@ Module X86Safe.
   similar_threadPool, but now we need a more invloved relation on
   cores that says that things may be more defined. Do we have one? *)
   
-  Parameter erasePool : FineConc.machine_state -> X86SC.machine_state -> Prop.
+  Inductive erasePool (tpf:FineConc.machine_state) (tpsc:X86SC.machine_state) : Prop :=
+  | ErasePool:
+        num_threads tpf = ErasedMachine.ThreadPool.num_threads tpsc ->
+        (forall i (pffi: containsThread tpf i)
+           (pfsci: ErasedMachine.ThreadPool.containsThread tpsc i),
+            getThreadC pffi = ErasedMachine.ThreadPool.getThreadC pfsci) ->
+        erasePool tpf tpsc.
+
+  (** The initial state of X86SC is an erasure of the initial state of
+  the FineConc machine *)
+  Lemma init_erasure:
+    forall f arg U tpsc tpf
+      (HinitSC: sc_init f arg = Some (U, [::], tpsc))
+      (HinitF: tpf_init f arg = Some (U, [::], tpf)),
+      erasePool tpf tpsc.
+  Proof.
+    intros.
+    unfold sc_init, tpf_init in *.
+    simpl in *. unfold X86SC.init_machine, FineConc.init_machine in *.
+    unfold init_mach, ErasedMachine.init_mach in *.
+    simpl in *.
+    destruct (Asm_initial_core the_ge f arg); try discriminate.
+    destruct init_perm; try discriminate.
+    inv HinitSC. inv HinitF.
+    unfold initial_machine, ErasedMachine.initial_machine.
+    simpl.
+    econstructor; simpl; eauto.
+  Qed.
+    
   (** Erasure from FineConc to X86-SC.*)
   Conjecture x86sc_erasure:
     forall sched f arg U tpsc tpf m trace
@@ -58,12 +86,42 @@ Module X86Safe.
 
   (** Competing Events *)
   
-  (* Definition compete (ev1 ev2 : machine_event) (tr : event_trace) : Prop := *)
-  (*   exists n m, *)
-  (*     List.nth_error tr n = Some ev1 /\ *)
-  (*     List.nth_error tr m = Some ev2 /\ *)
-  (*     thread_id ev1 <> thread_id ev2 /\ *)
-      
+  Definition competes (ev1 ev2 : machine_event) : Prop :=
+    thread_id ev1 <> thread_id ev2 /\
+    location ev1 = location ev2 /\
+    (is_internal ev1 ->
+     is_internal ev2 ->
+     action ev1 = Some Write \/ action ev2 = Some Write) /\
+    (is_external ev1 \/ is_external ev2 ->
+     action ev1 = Some Mklock \/ action ev1 = Some Freelock
+     \/ action ev2 = Some Mklock \/ action ev2 = Some Freelock).
+
+  (** Spinlock well synchronized*)
+  Definition spinlock_synchronized (tr : X86SC.event_trace) :=
+    forall i j ev1 ev2,
+      i < j ->
+      List.nth_error tr i = Some ev1 ->
+      List.nth_error tr j = Some ev2 ->
+      competes ev1 ev2 ->
+      exists u v eu ev,
+        i < u < v < j /\
+        List.nth_error tr u = Some eu /\
+        List.nth_error tr v = Some ev /\
+        action eu = Some Release /\ action ev = Some Acquire /\
+        location eu = location ev.
+
+  (** Spinlock clean *)
+  Definition spinlock_clean (tr : X86SC.event_trace) :=
+    forall i j evi evj,
+      i < j ->
+      List.nth_error tr i = Some evi ->
+      List.nth_error tr j = Some evj ->
+      action evi = Some Mklock ->
+      (~ exists u evu, i < u < j /\ List.nth_error tr u = Some evu /\
+                  action evu = Some Freelock /\ location evu = location evi) ->
+      location evj = location evi ->
+      action evj <> Some Write /\ action evj <> Some Read.
+  
 End X86Safe.
 
   
